backend/Constpropproof.v
@@ -22,6 +22,7 @@ Require Import ConstpropOp ConstpropOpproof Constprop.
 Definition match_prog (prog tprog: program) :=
   match_program (fun cu f tf => tf = transf_fundef (romem_for cu) f) eq prog tprog.
 
+#[global]
 Instance comp_transf_function rm: has_comp_transl (transf_function rm).
 Proof. now intro. Qed.
 
