cfrontend/Csharpminor.v
@@ -90,6 +90,7 @@ Record function : Type := mkfunction {
   fn_body: stmt
 }.
 
+#[global]
 Instance has_comp_function : has_comp function := fn_comp.
 
 Definition fundef := AST.fundef function.
